<link href="../whirlwind.css" rel="stylesheet">

<whirlheader>
<p>name</p>
<p>3D+1D</p>
<p>date</p>
</whirlheader>

# Basics 

This is our basis for the 3D Heisenberg Lie Algebra
$$
\begin{bmatrix}
0 & 1 & 0 \\
0 & 0 & 0 \\
0 & 0 & 0
\end{bmatrix}
,
\begin{bmatrix}
0 & 0 & 0 \\
0 & 0 & 1 \\
0 & 0 & 0
\end{bmatrix}
,
\begin{bmatrix}
0 & 0 & 1 \\
0 & 0 & 0 \\
0 & 0 & 0
\end{bmatrix}
$$

# 3D+1D Extension:

There are 3 possibilities:

## $\mathfrak{s}_{3,1}^{0,1}$

$\mathfrak{s}_{3,1}^{0,1}$ is defined by
$$


\begin{bmatrix}
2 & 0 & 0 \\
0 & 1 & 1 \\
0 & 0 & 1
\end{bmatrix}.
$$
Then 
$$
Q_{\mathfrak{s}_{3,1}^{0,1}}(z) = z_0^2 (z_0 + z_4)^2
$$
so 
$$
k(\mathfrak{s}_{3,1}^{0,1})=2.
$$

## $\mathfrak{s}_{3,1}^{0,2}$

$\mathfrak{s}_{3,1}^{0,2}$ is defined by
$$

\begin{bmatrix}
0 & 0 & 0 \\
0 & 1 & 0 \\
0 & 0 & -1
\end{bmatrix}
$$
Then 
$$
Q_{\mathfrak{s}_{3,1}^{0,2}}(z) = z_0 (z_0 - z_4)(z_0 + z_4)(z_0 + 2z_4)
$$
so 
$$
k(\mathfrak{s}_{3,1}^{0,2})=4.
$$

## $\mathfrak{s}_{3,1}^{1,1}$

$\mathfrak{s}_{3,1}^{1,1}$ is defined by
$$


\begin{bmatrix}
2 & 0 & 0 \\
0 & b+1 & 0 \\
0 & 0 & 1-b
\end{bmatrix}
$$
where $b \ge 0$.

Then
$$
Q_{\mathfrak{s}_{3,1}^{1,1,b}}(z)=z_0(z_0 + 2bz_4)(z_0 + (-b+1)z_4)(z_0 + (b+1)z_4)
$$

For there to be repeated roots, we must have duplicates in the set 
$$
\text{dup}\{0, 2b, -b+1, b+1 | b\ge 0\} \implies b=0, \frac{1}{3}, 1
$$

Then 
$$
k(\mathfrak{s}_{3,1}^{1,1,b}) = \begin{cases} 2& \text{if }b=0,1 \\ 
3 & \text{if } b=\frac{1}{3}\\ 
4& \text{otherwise}\end{cases}
$$

# Spectral Equivalence

We claim that there are $\infty=1+1+\infty$ many spectral equivalence classes:
- $k(L)=2$: $1$
- $k(L)=3$: $1$
- $k(L)=4$: $\infty$

## $k=2$

<proposition>

There is 1 spectral equivalence class.

</proposition>

<proof>

We have two cases to compare:
- $Q_{\mathfrak{s}_{3,1}^{0,1}}(z) =Q_{\mathfrak{s}_{3,1}^{1,1,0}}(z)=z_0^2(z_0 + z_4)^2$
- $Q_{\mathfrak{s}_{3,1}^{1,1,1}}(z)=z_0(z_0 + 2z_4)^2$
 
$$
B= \begin{bmatrix}
1 & 0 & 0 & 0 & 0 \\
0 & 1 & 0 & 0 & 0 \\
0 & 0 & 1 & 0 & 0 \\
0 & 0 & 0 & 1 & 0 \\
0 & 0 & 0 & 0 & \frac{1}{2}
\end{bmatrix}
$$
works, so the two Lie algebras are spectrally equivalent.

</proof>

## $k=3$

For $k=3$, there is only 1 case: $\mathfrak{s}_{3,1}^{1,1,\frac{1}{3}}$, so there is only 1 spectral equivalence class.

## $k=4$

For $k=4$, there are two cases 
- $Q_{\mathfrak{s}_{3,1}^{0,2}}(z) = z_0 (z_0 - z_4)(z_0 + z_4)(z_0 + 2z_4)$
- $Q_{\mathfrak{s}_{3,1}^{1,1,b}}(z)=z_0(z_0 + 2bz_4)(z_0 + (-b+1)z_4)(z_0 + (b+1)z_4)$

<proposition>

$\mathfrak{s}_{3,1}^{1,1,b} \stackrel{\text{SE}}{\cong} \mathfrak{s}_{3,1}^{1,1,b'} \Longleftrightarrow b=b'$

</proposition>

<proposition>

$\mathfrak{s}_{3,1}^{0,2} \stackrel{\text{SE}}{\not\cong}\mathfrak{s}_{3,1}^{1,1,b}$

</proposition>

We have $\infty$ many cases.

# Interesting Case

<proposition>

$\mathfrak{s}_{3,1}^{1,1,0} \stackrel{\text{SE}}{\equiv} \mathfrak{s}_{\dim \mathfrak{h}, \dim f}^{1,1,1}$ but $\mathfrak{s}_{3,1}^{1,1,0} \not\cong \mathfrak{s}_{\dim \mathfrak{h}, \dim f}^{1,1,1}$.

</proposition>

<proof>

Let $Q_{\mathfrak{s}_{3,1}^{1,1,0}}(z)=z_0^2(z_0+z_4)^2$ and $Q_{\mathfrak{s}_{3,1}^{1,1,1}}(z)=z_0^2(z_0+2z_4)^2$. It suffices to show the existence of a non-singular matrix $B$ such that 
$$
Q_{\mathfrak{s}_{3,1}^{1,1,0}}(z)=Q_{\mathfrak{s}_{3,1}^{1,1,1}}(zB).
$$
In particular, 
$$
B= \begin{bmatrix}
1 & 0 & 0 & 0 & 0 \\
0 & 1 & 0 & 0 & 0 \\
0 & 0 & 1 & 0 & 0 \\
0 & 0 & 0 & 1 & 0 \\
0 & 0 & 0 & 0 & \frac{1}{2}
\end{bmatrix}
$$
works, so the two Lie algebras are spectrally equivalent.

</proof>
